Foundation/Modal/PLoN/Logic/N.lean
@@ -6,30 +6,28 @@ namespace LO.Modal
 
 open PLoN
 open Formula.PLoN
+open Hilbert.PLoN
 open Modal.Entailment
 
 namespace PLoN
 
 abbrev AllFrameClass : PLoN.FrameClass := Set.univ
 
-instance : AllFrameClass.IsNonempty := by
-  use ⟨Unit, λ _ _ _ => True⟩;
-  tauto;
-
 end PLoN
 
 
 namespace N
 
-instance : AllFrameClass.DefinedBy Modal.N.axioms.instances := ⟨by simp⟩
+instance PLoN.sound : Sound Modal.N PLoN.AllFrameClass := instFrameClassSound $ by
+  constructor;
+  grind;
 
-instance PLoN.sound : Sound Modal.N PLoN.AllFrameClass := inferInstance
+instance : Entailment.Consistent Modal.N := consistent_of_nonempty_frameClass PLoN.AllFrameClass $ by
+  use PLoN.terminalFrame;
+  tauto;
 
-instance : Entailment.Consistent Modal.N := PLoN.Hilbert.consistent_of_FrameClass PLoN.AllFrameClass
-
-instance : Canonical Modal.N PLoN.AllFrameClass := ⟨by tauto⟩
-
-instance PLoN.complete : Complete Modal.N PLoN.AllFrameClass := inferInstance
+instance PLoN.complete : Complete Modal.N PLoN.AllFrameClass := instComplete_of_mem_canonicalFrame $ by
+  tauto;
 
 end N
 
@@ -49,7 +47,7 @@ instance : Modal.N ⪱ Modal.EN := by
     . apply re!;
       cl_prover;
     . apply Sound.not_provable_of_countermodel (𝓜 := PLoN.AllFrameClass);
-      apply Formula.PLoN.ValidOnFrameClass.not_of_exists_model;
+      apply not_validOnFrameClass_of_exists_model;
       use {
         World := Fin 2,
         Rel ξ x y := if ξ = ∼∼(.atom 0) then True else False,
@@ -57,7 +55,7 @@ instance : Modal.N ⪱ Modal.EN := by
       };
       constructor;
       . tauto;
-      . simp [Semantics.Models, ValidOnModel, Satisfies, Frame.Rel'];
+      . simp [Frame.Rel'];
 
 
 instance : Modal.N ⪱ Modal.K := by
@@ -68,7 +66,7 @@ instance : Modal.N ⪱ Modal.K := by
     constructor;
     . simp;
     . apply Sound.not_provable_of_countermodel (𝓜 := PLoN.AllFrameClass)
-      apply Formula.PLoN.ValidOnFrameClass.not_of_exists_model;
+      apply not_validOnFrameClass_of_exists_model;
       use {
         World := Fin 2,
         Rel := λ ξ x y =>
@@ -83,24 +81,6 @@ instance : Modal.N ⪱ Modal.K := by
       };
       constructor;
       . tauto;
-      . simp only [ValidOnModel.iff_models, ValidOnModel, not_forall];
-        use 0;
-        apply Formula.PLoN.Satisfies.imp_def.not.mpr;
-        push_neg;
-        constructor;
-        . intro x R0x;
-          simp_all [Satisfies, Frame.Rel'];
-        . apply Formula.PLoN.Satisfies.imp_def.not.mpr;
-          push_neg;
-          constructor;
-          . intro x R0x;
-            simp_all [Satisfies, Frame.Rel'];
-            omega;
-          . apply Satisfies.box_def.not.mpr;
-            push_neg;
-            use 1;
-            constructor;
-            . simp [Frame.Rel']
-            . simp [Semantics.Models, Satisfies];
+      . simp [Frame.Rel'];
 
 end LO.Modal
