Foundation/Modal/PLoN/Hilbert.lean
@@ -7,41 +7,36 @@ open PLoN
 open Formula
 open Formula.PLoN
 
-namespace PLoN.Hilbert
+namespace Hilbert.PLoN
 
 open Formula
 
 variable {Ax : Axiom ℕ} {φ : Formula ℕ}
 variable {F : Frame} {C : FrameClass}
 
-lemma soundness_of_defined_by_AxiomInstances [defined : C.DefinedBy Ax.instances] : Hilbert.Normal Ax ⊢ φ → C ⊧ φ := by
+lemma soundness_frameclass (hV : C ⊧* Ax.instances) : Hilbert.Normal Ax ⊢ φ → C ⊧ φ := by
   intro hφ F hF;
   induction hφ using Hilbert.Normal.rec! with
-  | @axm φ s h =>
-    apply defined.defines F |>.mp hF;
-    use φ;
-    tauto;
-  | mdp ihpq ihp => exact ValidOnFrame.mdp ihpq ihp;
-  | nec ih => exact ValidOnFrame.nec ih;
-  | implyK => exact ValidOnFrame.implyK;
-  | implyS => exact ValidOnFrame.implyS;
-  | ec => exact ValidOnFrame.elimContra;
+  | axm s h =>
+    apply hV.models;
+    . grind;
+    . assumption;
+  | mdp ihpq ihp =>
+    intro V;
+    apply ValidOnModel.mdp (ihpq V) (ihp V);
+  | _ => grind;
 
-instance [C.DefinedBy Ax.instances] : Sound (Hilbert.Normal Ax) C := ⟨fun {_} => soundness_of_defined_by_AxiomInstances⟩
+instance instFrameClassSound (hV : C ⊧* Ax.instances) : Sound (Hilbert.Normal Ax) C := ⟨fun {_} => soundness_frameclass hV⟩
 
-lemma consistent_of_FrameClass_aux [nonempty : C.IsNonempty] [sound : Sound (Hilbert.Normal Ax) C] : (Hilbert.Normal Ax) ⊬ ⊥ := by
+lemma consistent_of_nonempty_frameClass (C : PLoN.FrameClass) (hC : Set.Nonempty C) [sound : Sound (Hilbert.Normal Ax) C] : Entailment.Consistent (Hilbert.Normal Ax) := by
+  apply Entailment.Consistent.of_unprovable (φ := ⊥);
   apply not_imp_not.mpr sound.sound;
-  apply ValidOnFrameClass.not_of_exists_frame;
-  obtain ⟨F, hF⟩ := nonempty;
+  apply Semantics.set_models_iff.not.mpr;
+  push_neg;
+  obtain ⟨F, hF⟩ := hC;
   use F;
-  constructor;
-  . assumption;
-  . simp;
+  grind;
 
-lemma consistent_of_FrameClass (C : PLoN.FrameClass) [C.IsNonempty] [Sound (Hilbert.Normal Ax) C] : Entailment.Consistent (Hilbert.Normal Ax) := by
-  apply Entailment.Consistent.of_unprovable;
-  exact consistent_of_FrameClass_aux (C := C);
-
-end PLoN.Hilbert
+end Hilbert.PLoN
 
 end LO.Modal
